IMP--_To_SAS+/SAS_Plus_Plus_To_SAS_Plus.thy
@@ -1,0 +1,257 @@
+\<^marker>\<open>creator Florian Keßler\<close>
+
+section "SAS++ to SAS+"
+
+theory SAS_Plus_Plus_To_SAS_Plus imports SAS_Plus_Plus
+begin 
+
+datatype 'v variable =  Var 'v | Stage
+datatype 'd domain_element = DE 'd | Init | NonInit
+                                                               
+type_synonym ('v, 'd) state = "('v, 'd) State_Variable_Representation.state"
+type_synonym ('v, 'd) operator = "('v variable, 'd domain_element) sas_plus_operator"
+type_synonym ('v, 'd) problem = "('v variable, 'd domain_element) sas_plus_problem"
+
+definition SAS_Plus_Plus_State_To_SAS_Plus:: 
+  "('d domain_element \<times> ('v, 'd) state) \<Rightarrow> ('v variable, 'd domain_element) state" where
+"SAS_Plus_Plus_State_To_SAS_Plus is = ((\<lambda>x. Some (DE x)) \<circ>\<^sub>m (snd is)
+  \<circ>\<^sub>m (\<lambda>x. (case x of Var x \<Rightarrow> Some x | Stage \<Rightarrow> None)))(Stage \<mapsto> (fst is))"
+
+lemma SAS_Plus_Plus_State_To_SAS_Plus_eq_iff_snd_eq[simp]:
+  "SAS_Plus_Plus_State_To_SAS_Plus (i, s) = SAS_Plus_Plus_State_To_SAS_Plus (i, s') 
+  \<longleftrightarrow> s = s'" 
+  apply (auto simp: SAS_Plus_Plus_State_To_SAS_Plus_def map_comp_def fun_eq_iff 
+      split: option.splits variable.splits)
+  by (metis option.exhaust_sel)
+
+lemma SAS_Plus_Plus_State_To_SAS_Plus_update_stage[simp]:
+  "SAS_Plus_Plus_State_To_SAS_Plus (a, s)(Stage \<mapsto> b) = SAS_Plus_Plus_State_To_SAS_Plus (b, s)"
+  by (auto simp: SAS_Plus_Plus_State_To_SAS_Plus_def map_comp_def fun_eq_iff)
+
+lemma SAS_Plus_Plus_State_To_SAS_Plus_map_le[simp]: 
+  "SAS_Plus_Plus_State_To_SAS_Plus (a, s) \<subseteq>\<^sub>m m 
+    \<Longrightarrow> SAS_Plus_Plus_State_To_SAS_Plus (b, s) \<subseteq>\<^sub>m m(Stage \<mapsto> b)" 
+  by(auto simp: SAS_Plus_Plus_State_To_SAS_Plus_def map_le_def map_comp_def 
+      split: option.splits variable.splits)
+
+definition SAS_Plus_Plus_Operator_To_SAS_Plus_Operator:: 
+  "('v, 'd) sas_plus_operator \<Rightarrow> ('v, 'd) operator" where
+"SAS_Plus_Plus_Operator_To_SAS_Plus_Operator op = 
+  \<lparr> precondition_of = (Stage, NonInit) # (map (\<lambda> x. (Var (fst x), DE (snd x))) (precondition_of op)),
+    effect_of = (map (\<lambda> x. (Var (fst x), DE (snd x))) (effect_of op))\<rparr>"
+
+lemma dom_of_map_of_map[simp]: 
+  "dom (map_of (map (\<lambda>x. (Var (fst x), DE (snd x))) l)) = (\<lambda>x. Var (fst x)) ` set l" 
+  apply(induction l)
+  apply(auto)
+  by (metis (mono_tags, lifting) domD fst_conv imageI)
+
+lemma map_of_map_eq_None_iff[simp]: "(map_of (map (\<lambda>x. (Var (fst x), DE (snd x))) l) (Var y) = None)
+  \<longleftrightarrow> (y \<notin> fst ` set l)"
+  apply(induction l)
+  by(auto)
+
+lemma map_of_map_eq_Some_iff[simp]: "(map_of (map (\<lambda>x. (Var (fst x), DE (snd x))) l) (Var x) = Some (DE y))
+  \<longleftrightarrow> (map_of l x = Some y)"
+  apply(induction l)
+  by(auto)
+
+lemma SAS_Plus_Plus_Operator_To_SAS_Plus_Operator_applicable[simp]: 
+  "is_operator_applicable_in (SAS_Plus_Plus_State_To_SAS_Plus (i, s)) 
+    (SAS_Plus_Plus_Operator_To_SAS_Plus_Operator op)
+  \<longleftrightarrow> (i = NonInit \<and> is_operator_applicable_in s op)"
+  apply(auto simp: SAS_Plus_Plus_State_To_SAS_Plus_def map_comp_def 
+      SAS_Plus_Plus_Operator_To_SAS_Plus_Operator_def)
+    apply(simp_all add: map_le_def)
+   apply(auto split: option.splits variable.splits)
+  apply(frule map_of_SomeD)
+    apply auto
+  by (metis domI weak_map_of_SomeI)+
+
+lemma SAS_Plus_Plus_Operator_To_SAS_Plus_Operator_execute[simp]:
+  "SAS_Plus_Plus_State_To_SAS_Plus (i, s) ++ map_of (effect_of (SAS_Plus_Plus_Operator_To_SAS_Plus_Operator op))
+  = SAS_Plus_Plus_State_To_SAS_Plus(i, s \<then>\<^sub>+ op)" 
+  using map_of_SomeD
+  apply(auto simp: SAS_Plus_Plus_State_To_SAS_Plus_def map_comp_def fun_eq_iff map_add_def 
+      SAS_Plus_Plus_Operator_To_SAS_Plus_Operator_def split: option.splits variable.splits)
+  apply force+
+  prefer 9 using map_of_SomeD apply fastforce
+  using map_of_map_eq_None_iff map_of_map_eq_Some_iff
+  by (metis (mono_tags, lifting) map_of_eq_None_iff map_of_map_eq_Some_iff option.simps 
+      option.distinct domI  domIff option.simps)+
+
+lemma execute_SAS_Plus_Plus_ops_in_SAS_Plus[simp]:
+  "execute_serial_plan_sas_plus (SAS_Plus_Plus_State_To_SAS_Plus (NonInit, s))
+    (map SAS_Plus_Plus_Operator_To_SAS_Plus_Operator ops) 
+    = SAS_Plus_Plus_State_To_SAS_Plus (NonInit, execute_serial_plan_sas_plus s ops)"
+  apply(induction ops arbitrary: s)
+   apply(simp add: SAS_Plus_Plus_State_To_SAS_Plus_def 
+      SAS_Plus_Plus_Operator_To_SAS_Plus_Operator_def)
+  by(auto simp: SAS_Plus_Plus_Operator_To_SAS_Plus_Operator_applicable[simplified])
+
+definition initialization_operators:: "('v, 'd) sas_plus_problem \<Rightarrow> ('v, 'd) operator list" where
+"initialization_operators P = \<lparr> precondition_of = [], effect_of = [(Stage, NonInit)]\<rparr> #
+  concat (map (\<lambda> v. (if v \<in> dom ((P)\<^sub>I\<^sub>+) then [] 
+    else map (\<lambda> y. \<lparr> precondition_of = [(Stage, Init)],  effect_of = [(Var v, DE y)]\<rparr>) 
+      (the (range_of P v)))) ((P)\<^sub>\<V>\<^sub>+))"
+
+lemma in_initialization_operators_iff[simp]: 
+  "\<lparr>precondition_of = [(Stage, Init)], effect_of = [(Var x, DE y)]\<rparr> 
+    \<in> set (initialization_operators P) 
+  \<longleftrightarrow> (x \<in> set ((P)\<^sub>\<V>\<^sub>+) \<and> ((P)\<^sub>I\<^sub>+) x = None \<and> y \<in> set (the (range_of P x)))"
+  by(auto simp: initialization_operators_def)
+
+definition initial_state:: 
+  "('v, 'd) sas_plus_problem \<Rightarrow> ('v variable, 'd domain_element) state" where
+"initial_state P = (\<lambda> v.
+  (case v of 
+    Var var \<Rightarrow> (if var \<in> set ((P)\<^sub>\<V>\<^sub>+) then Some (DE (case ((P)\<^sub>I\<^sub>+) var of 
+        (Some val) \<Rightarrow> val |
+        None \<Rightarrow> (the (range_of P var)) ! 0))
+      else None) |
+    Stage \<Rightarrow> Some Init))"
+
+definition SAS_Plus_Plus_To_SAS_Plus:: "('v, 'd) sas_plus_problem \<Rightarrow> ('v, 'd) problem" where
+"SAS_Plus_Plus_To_SAS_Plus P = \<lparr> variables_of = Stage # (map Var ((P)\<^sub>\<V>\<^sub>+)),
+      operators_of = (initialization_operators P) 
+        @ (map SAS_Plus_Plus_Operator_To_SAS_Plus_Operator ((P)\<^sub>\<O>\<^sub>+)), 
+      initial_of = initial_state P ,
+      goal_of = SAS_Plus_Plus_State_To_SAS_Plus (NonInit, ((P)\<^sub>G\<^sub>+)),
+      range_of = ((\<lambda>x. Some (map DE x)) \<circ>\<^sub>m (range_of P) 
+        \<circ>\<^sub>m (\<lambda>x. (case x of Var x \<Rightarrow> Some x | Stage \<Rightarrow> None)))(Stage \<mapsto> [Init, NonInit])\<rparr>"
+
+lemma Var_not_in_map_Var_iff[simp]: "Var x \<notin> Var ` S \<longleftrightarrow> x \<notin> S" by auto
+
+lemma SAS_Plus_Plus_To_SAS_Plus_valid: 
+  assumes "is_valid_problem_sas_plus_plus P"
+  shows "is_valid_problem_sas_plus (SAS_Plus_Plus_To_SAS_Plus P)" 
+  using assms apply(auto simp: is_valid_problem_sas_plus_plus_def is_valid_problem_sas_plus_def 
+      SAS_Plus_Plus_To_SAS_Plus_def list_all_def is_valid_operator_sas_plus_def Let_def
+      initialization_operators_def SAS_Plus_Plus_Operator_To_SAS_Plus_Operator_def ListMem_iff)
+               apply auto
+              apply fastforce
+             apply fastforce
+            apply fastforce
+           apply fastforce
+          apply blast
+         apply blast
+         apply(auto simp: initial_state_def map_comp_def SAS_Plus_Plus_State_To_SAS_Plus_def 
+        split: variable.splits if_splits option.splits)
+  by (meson assms is_valid_problem_sas_plus_plus_then(1) range_of_not_empty)+
+
+lemma stage_of_initial_state[simp]: "((SAS_Plus_Plus_To_SAS_Plus P)\<^sub>I\<^sub>+) Stage = Some Init" 
+  by(auto simp: SAS_Plus_Plus_To_SAS_Plus_def initial_state_def)
+
+definition initialization_sequence:: "('v \<times> 'd) list \<Rightarrow> ('v, 'd) operator list" where
+  "initialization_sequence vs = map (\<lambda>v. \<lparr> precondition_of = [(Stage, Init)],  
+      effect_of = [(Var (fst v), DE (snd v))]\<rparr>) vs"
+
+lemma result_of_initialization_sequence[simp]: 
+  assumes "I Stage = Some Init"
+    "distinct (map fst vs)"
+  shows "execute_serial_plan_sas_plus I (initialization_sequence vs) = 
+  I ++ SAS_Plus_Plus_State_To_SAS_Plus (Init, map_of vs)"
+using assms proof (induction vs arbitrary: I)
+  case Nil
+  then show ?case using Nil
+    by (auto simp: initialization_sequence_def SAS_Plus_Plus_State_To_SAS_Plus_def map_add_def)
+next
+  case (Cons v vs)
+  hence "execute_serial_plan_sas_plus I (initialization_sequence (v # vs)) 
+    = execute_serial_plan_sas_plus (I(Var (fst v) \<mapsto> DE (snd v))) (initialization_sequence vs)"
+    by (auto simp: initialization_sequence_def map_le_def)
+  also have "... = I ++ SAS_Plus_Plus_State_To_SAS_Plus (Init, map_of (v # vs))" using Cons
+    by(auto simp: SAS_Plus_Plus_State_To_SAS_Plus_def map_add_def fun_eq_iff map_comp_def 
+        rev_image_eqI split: option.splits variable.splits)
+  ultimately show ?case by metis
+qed
+
+lemma initialization_sequence_chain_applicable_condition[simp]:
+  assumes "s Stage = Some Init"
+  shows "chain_applicable s (initialization_sequence vs)"
+  using assms apply(induction vs arbitrary: s)
+  by(auto simp:  initialization_sequence_def map_le_def)
+
+lemma map_of_conact_map_cases_eq_Some[simp]: 
+  "map_of (concat (map (\<lambda>v. case m v of None \<Rightarrow> [(v, f v)] | Some x \<Rightarrow> []) l)) x = Some y 
+  \<longleftrightarrow> (x \<in> set l \<and> f x = y \<and> m x = None)"
+proof
+  assume "map_of (concat (map (\<lambda>v. case m v of None \<Rightarrow> [(v, f v)] | Some x \<Rightarrow> []) l)) x = Some y" 
+  then show "x \<in> set l \<and> f x = y \<and> m x = None"  
+    apply -
+    apply(drule map_of_SomeD)
+    by(auto)
+next
+  assume "x \<in> set l \<and> f x = y \<and> m x = None"
+  hence "(x, y) \<in> set (concat (map (\<lambda>v. case m v of None \<Rightarrow> [(v, f v)] | Some x \<Rightarrow> []) l))"
+    by auto
+  moreover have "\<forall>y'. (x, y') \<in> set (concat (map (\<lambda>v. case m v of None \<Rightarrow> [(v, f v)] | Some x \<Rightarrow> []) l))
+    \<longrightarrow> y' = f x" by auto
+  ultimately show "map_of (concat (map (\<lambda>v. case m v of None \<Rightarrow> [(v, f v)] | Some x \<Rightarrow> []) l)) x = Some y"
+    by (metis (no_types, lifting) map_of_SomeD weak_map_of_SomeI)
+qed
+
+lemma map_of_conact_map_cases_eq_None[simp]: 
+  "map_of (concat (map (\<lambda>v. case m v of None \<Rightarrow> [(v, f v)] | Some x \<Rightarrow> []) l)) x = None 
+  \<longleftrightarrow> (x \<notin> set l \<or> m x \<noteq> None)"
+proof -
+  have "(map_of (concat (map (\<lambda>v. case m v of None \<Rightarrow> [(v, f v)] | Some x \<Rightarrow> []) l)) x = None)
+    = (\<not>(\<exists>y. map_of (concat (map (\<lambda>v. case m v of None \<Rightarrow> [(v, f v)] | Some x \<Rightarrow> []) l)) x = Some y))"
+    by fastforce
+  also have "... = (\<not>(\<exists>y. x \<in> set l \<and> f x = y \<and> m x = None))" by auto
+  ultimately show ?thesis by simp
+qed
+
+lemma distinct_map_fst_concat[simp]:
+  "distinct (map fst (concat (map (\<lambda>v. case m v of None \<Rightarrow> [(v, f v)] | Some x \<Rightarrow> []) (remdups l))))"
+  apply(induction l) 
+  by(auto split: option.splits)
+
+lemma length_concat_map[simp]: 
+  "length (concat (map (\<lambda>v. case m v of None \<Rightarrow> [f v] | Some _ \<Rightarrow> []) (remdups l))) \<le> length l"
+  apply(induction l)
+  by(auto split: option.splits)
+
+lemma SAS_Plus_Plus_To_SAS_Plus:
+  assumes "is_valid_problem_sas_plus_plus P" 
+    "is_serial_solution_for_problem_sas_plus_plus P plan"
+  shows "\<exists>prefix. length prefix \<le> length ((P)\<^sub>\<V>\<^sub>+) + 1 
+    \<and> is_serial_solution_for_problem (SAS_Plus_Plus_To_SAS_Plus P) 
+        (prefix @ (map SAS_Plus_Plus_Operator_To_SAS_Plus_Operator plan))" 
+proof -
+  obtain I where I_def: "((P)\<^sub>I\<^sub>+) \<subseteq>\<^sub>m I \<and> dom I = set ((P)\<^sub>\<V>\<^sub>+)
+        \<and> (\<forall> v \<in> set ((P)\<^sub>\<V>\<^sub>+). the (I v) \<in> range_of' P v)
+        \<and> ((P)\<^sub>G\<^sub>+) \<subseteq>\<^sub>m execute_serial_plan_sas_plus I plan
+        \<and> list_all (\<lambda>op. ListMem op ((P)\<^sub>\<O>\<^sub>+)) plan" using assms 
+    by (auto simp: is_serial_solution_for_problem_sas_plus_plus_def Let_def)
+  let ?P' = "SAS_Plus_Plus_To_SAS_Plus P"
+  let ?missing_vs = "(concat (map (\<lambda>v. case ((P)\<^sub>I\<^sub>+) v of Some _ \<Rightarrow> [] |
+    None \<Rightarrow> [(v, the (I v))]) (remdups ((P)\<^sub>\<V>\<^sub>+))))"
+  let ?prefix' = "initialization_sequence ?missing_vs"
+  let ?prefix = "?prefix' @ [\<lparr> precondition_of = [], effect_of = [(Stage, NonInit)]\<rparr>]"
+  have "execute_serial_plan_sas_plus ((?P')\<^sub>I\<^sub>+) ?prefix' 
+    = SAS_Plus_Plus_State_To_SAS_Plus (Init, I)" using I_def
+    apply(auto simp: SAS_Plus_Plus_To_SAS_Plus_def SAS_Plus_Plus_State_To_SAS_Plus_def map_le_def
+        initial_state_def map_add_def map_comp_def fun_eq_iff split: option.splits variable.splits)
+    by (metis domI option.inject)
+  hence "execute_serial_plan_sas_plus ((?P')\<^sub>I\<^sub>+) 
+    (?prefix @ (map SAS_Plus_Plus_Operator_To_SAS_Plus_Operator plan)) 
+    = SAS_Plus_Plus_State_To_SAS_Plus (NonInit, execute_serial_plan_sas_plus I plan)" by auto
+  hence "((?P')\<^sub>G\<^sub>+) \<subseteq>\<^sub>m execute_serial_plan_sas_plus ((?P')\<^sub>I\<^sub>+) 
+    (?prefix @ (map SAS_Plus_Plus_Operator_To_SAS_Plus_Operator plan))" using I_def 
+    apply(auto simp:  SAS_Plus_Plus_To_SAS_Plus_def SAS_Plus_Plus_State_To_SAS_Plus_def 
+        map_add_def map_comp_def split: option.splits variable.splits)
+    apply(simp add: map_le_def fun_eq_iff)
+    by (metis (no_types, lifting) domIff option.case_eq_if)
+  hence "length ?prefix \<le> length ((P)\<^sub>\<V>\<^sub>+) + 1 
+    \<and> is_serial_solution_for_problem (SAS_Plus_Plus_To_SAS_Plus P) 
+        (?prefix @ (map SAS_Plus_Plus_Operator_To_SAS_Plus_Operator plan))"
+    using I_def
+    apply(auto simp: is_serial_solution_for_problem_def Let_def list_all_def 
+        initialization_sequence_def ListMem_iff SAS_Plus_Plus_To_SAS_Plus_def range_of'_def 
+        split: option.splits)
+    by (simp add: initialization_operators_def)
+  then show ?thesis by blast
+qed
+
+end
